Syntax.v
@@ -157,9 +157,10 @@ Section Phoas.
     Variable k: Kind.
     Variable arr: Expr (Array n k).
     Definition ArrayReverse: Expr (Array n k).
-      refine (BuildArray (@Build_SameTuple _ n (map (fun i => ReadArrayConst arr i) (rev (genFinType n)))
+      refine (BuildArray (@Build_SameTuple _ n (map (fun i => ReadArrayConst arr i) (rev_tail (genFinType n) nil))
                             (transparent_Is_true _ _))).
       Proof.
+        rewrite rev_tail_fast.
         rewrite length_map, length_rev, genFinType_length, Nat.eqb_refl; auto.
       Defined.
   End ArrayReverse.
